%%%
\documentclass[a4paper,11pt,twoside]{report}
%%%
\input{../preamble.tex}
%%%
\begin{document}

\LARGE\textsc{Date: 2020-09-22} \\ \\ \LARGE\textsc{Announcements:} \\
\small



\paragraph \hrule \paragraph \\ \fancyhead[R]{Lesson 16} \fancyhead[L]{Week 4}
%  %  %  %  %  %  %  %  %  %  %  %  %  %  %  %  %  %  %  %  %  %  %  %  %  %  %  %
\section{The Chain Rule}%
\label{sec:the_chain_rule}

\[y = f(g(x))\]

let
\begin{align*}
	u = g(x) &\to \frac{\partial u}{\partial x} = g'(x) \\
	y = f(u) &\to \frac{\partial y}{\partial u} = f'(u) \\
\end{align*}

\subsection{The Chain Rule (Case 1)}%
\label{sub:the_chain_rule_case_1_}

Suppose $z = f(x,y)$ is a differentiable function of $x$ and $y$, where $x$ and $y$ are
differentiable functions of $t$, Then $z$ is a differentiable function of $t$ and \[
\frac{dz}{dt} = \frac{\partial z}{\partial x} \cdot \frac{d x}{d t} + \frac{\partial z}{\partial y}\cdot \frac{d y}{d t} \]


\begin{example}[Case 1 Chain Rule]
	\begin{align*}
	z&= x^2y + 3x^3y^{4} \\
	x&= e^{2t} \\
	y&= \cos t \\
	\end{align*}
	\begin{align*}
		\frac{\partial z}{\partial x} &=  2xy + 9 x^2 y^{4} \\
		\frac{\partial z}{\partial y} &=  x^2 + 12 x^3 y^{3} \\
	\end{align*}
	\begin{align*}
		\frac{dx}{dt}&= 2e^{2t}\\
		\frac{dy}{dt}&= -\sin t \\
	\end{align*}

	\begin{align*}
		\frac{dz}{dt} &= (2xy + 9x^2y^{4})2e^{2t} + (x^2 + 12x^3y^3)\cdot -\sin t \\
	\end{align*}
\smallskip\hfill$\bullet$\end{example}

\subsection{The Chain Rule (Case 2)}%
\label{sub:the_chain_rule_case_2_}

Suppose $z = f(x,y)$ is a differentiable function of $x$ and $y$, where $x= g(s,t)$ and $y = h(s,t)$ are
differentiable functions of $t$, Then $z$ is a differentiable function of $s$ and $t$, Then








%  %  %  %  %  %  %  %  %  %  %  %  %  %  %  %  %  %  %  %  %  %  %  %  %  %  %  %
\newpage
%%%
\end{document}

%LEAVE EMPTY ROW ABOVE THIS ONE
